# baseURI: http://linked.data.gov.au/def/auspix
# imports: http://linked.data.gov.au/def/geox
# prefix: apo

@prefix apo: <http://linked.data.gov.au/def/auspix#> .
@prefix auspix: <http://pid.geoscience.gov.au/dggs/ausPIX/> .
@prefix data: <http://linked.data.gov.au/def/datatype/> .
@prefix dcterms: <http://purl.org/dc/terms/> .
@prefix geo: <http://www.opengis.net/ont/geosparql#> .
@prefix geox: <http://linked.data.gov.au/def/geox#> .
@prefix owl: <http://www.w3.org/2002/07/owl#> .
@prefix rdf: <http://www.w3.org/1999/02/22-rdf-syntax-ns#> .
@prefix rdfs: <http://www.w3.org/2000/01/rdf-schema#> .
@prefix sdo: <http://schema.org/> .
@prefix skos: <http://www.w3.org/2004/02/skos/core#> .
@prefix xsd: <http://www.w3.org/2001/XMLSchema#> .

<http://catalogue.linked.data.gov.au/org/csiro>
  a sdo:Organization ;
  sdo:identifier <https://ror.org/03qn8fb07> ;
  sdo:mainEntityOfPage <https://www.csiro.au/> ;
  sdo:name "CSIRO" ;
.
<http://linked.data.gov.au/def/auspix>
  a owl:Ontology ;
  dcterms:created "2020-02-05"^^xsd:date ;
  dcterms:creator <https://orcid.org/0000-0002-3884-3420> ;
  dcterms:modified "2020-05-25"^^xsd:date ;
  rdfs:comment """An ontology to allow AusPIX objects to be linked into Loc-I. 

Two classes are defined: a `AusPIX CellAggregate` is composed of one or more `AusPIX Cells`. 

An AusPIX CellAggregate may be used to provide a geometrical approximation for other Loc-I Features using the (loci|apo):equivalent predicate. """ ;
  rdfs:label "AusPIX Ontology" ;
  rdfs:seeAlso <http://www.opengis.net/doc/AS/dggs/1.0> ;
  rdfs:seeAlso <https://github.com/GeoscienceAustralia/AusPIX_DGGS> ;
  owl:imports <http://linked.data.gov.au/def/geox> ;
.
apo:Cell
  a owl:Class ;
  rdfs:comment """Cell, from [AusPIX](https://github.com/GeoscienceAustralia/AusPIX-DGGS-dataset)

Individual cells should be refered to using an IRI, typically a call to the AusPIX service.""" ;
  rdfs:label "AusPIX Cell" ;
  rdfs:subClassOf geo:Feature ;
  rdfs:subClassOf [
      a owl:Restriction ;
      owl:allValuesFrom apo:Cell ;
      owl:onProperty apo:hasNeighbourDown ;
    ] ;
  rdfs:subClassOf [
      a owl:Restriction ;
      owl:allValuesFrom apo:Cell ;
      owl:onProperty apo:hasNeighbourLeft ;
    ] ;
  rdfs:subClassOf [
      a owl:Restriction ;
      owl:allValuesFrom apo:Cell ;
      owl:onProperty apo:hasNeighbourRight ;
    ] ;
  rdfs:subClassOf [
      a owl:Restriction ;
      owl:allValuesFrom apo:Cell ;
      owl:onProperty apo:hasNeighbourUp ;
    ] ;
  rdfs:subClassOf [
      a owl:Restriction ;
      owl:cardinality "1"^^xsd:nonNegativeInteger ;
      owl:onProperty geox:hasCentroid ;
    ] ;
  rdfs:subClassOf [
      a owl:Restriction ;
      owl:minCardinality "1"^^xsd:nonNegativeInteger ;
      owl:onProperty geox:hasArea ;
    ] ;
  rdfs:subClassOf [
      a owl:Restriction ;
      owl:minCardinality "1"^^xsd:nonNegativeInteger ;
      owl:onProperty dcterms:identifier ;
    ] ;
  rdfs:subClassOf [
      a owl:Restriction ;
      owl:minCardinality "1"^^xsd:nonNegativeInteger ;
      owl:onProperty geo:hasGeometry ;
    ] ;
  rdfs:subClassOf [
      a owl:Restriction ;
      owl:minCardinality "1"^^xsd:nonNegativeInteger ;
      owl:onProperty geo:sfWithin ;
    ] ;
  rdfs:subClassOf [
      a owl:Restriction ;
      owl:minCardinality "9"^^xsd:nonNegativeInteger ;
      owl:onProperty geo:sfContains ;
    ] ;
  skos:example """
auspix:R7852 a apo:Cell ;
  dcterms:identifier 'R7852' ;
  apo:upNeighbour apo:R7828 ;
  apo:downNeighbour apo:R7855 ;
  apo:rightNeighbour apo:R8630 ;
  apo:leftNeighbour apo:R7851 ;
  geo:hasGeometry 'POLYGON ((148.88888888888889 -34.663795228918765, 150.0 -34.663795228918765, 150.0 -35.81859718358464, 148.88888888888889 -35.81859718358464))'^^geo:wktLiteral ;
  geo:sfContains apo:R78520 , apo:R78521 , apo:R78522 , apo:R78523 , apo:R78524 , apo:R78525 , apo:R78526 , apo:R78527 , apo:R78528 ; 
  geo:sfWithin apo:R785 ; 
  geox:centroid 'POINT (149.44444444444443 -35.23915910922053)'^^geo:wktLiteral ;
  geox:hasAreaM2 [ data:value 12971551595.0 ] ; 
.
""" ;
.
apo:CellAggregate
  a owl:Class ;
  rdfs:comment "An AusPIX CellAggregate is composed of a set of auspix Cells" ;
  rdfs:label "AusPIX CellAggregate" ;
  rdfs:subClassOf geo:Feature ;
  rdfs:subClassOf [
      a owl:Restriction ;
      owl:allValuesFrom apo:Cell ;
      owl:onProperty rdfs:member ;
    ] ;
  rdfs:subClassOf [
      a owl:Restriction ;
      owl:minCardinality "1"^^xsd:nonNegativeInteger ;
      owl:onProperty rdfs:member ;
    ] ;
  skos:example """
auspix:Agg_1
  rdf:type apo:CellAggregate ;
  dcterms:identifier 'Agg_1' ;
  rdfs:member apo:R7828 ;
  rdfs:member apo:R78520 ;
  rdfs:member apo:R78521 ;
  rdfs:member apo:R78522 ;
  rdfs:member apo:R78523 ;
.
""" ;
.
apo:equivalent
  a owl:ObjectProperty ;
  rdfs:comment """This property is used to relate an individual feature from one geography or dataset with a feature from another geography or dataset which is intended to represent the same real-world entity.

Use of (loci|apo):equivalent would allow representations using slightly different geometrical bases (e.g. surveyed geometries, aggregates of DGGS cells, aggregates of ASGS meshblocks) to be linked, in situations where a purely geometrical computation might not get to a `geo:sfEquals` relationships because of differing precision, slivers, etc,. When the data provider's intention is that they match, then this predicate can be used to make that assertion. The provenance of the assertion maybe be recorded in the usual way in a link-set.""" ;
  rdfs:domain geo:Feature ;
  rdfs:label "equivalent to" ;
  rdfs:range geo:Feature ;
.
apo:hasNeighbourDown
  a owl:ObjectProperty ;
  rdfs:label "has neighbour downward" ;
  rdfs:subPropertyOf geo:sfTouches ;
.
apo:hasNeighbourLeft
  a owl:ObjectProperty ;
  rdfs:label "has neighbour to the left" ;
  rdfs:subPropertyOf geo:sfTouches ;
.
apo:hasNeighbourRight
  a owl:ObjectProperty ;
  rdfs:label "has neighbour to the right" ;
  rdfs:subPropertyOf geo:sfTouches ;
.
apo:hasNeighbourUp
  a owl:ObjectProperty ;
  rdfs:label "has neighbour upward" ;
  rdfs:subPropertyOf geo:sfTouches ;
.
auspix:Agg_1
  a apo:CellAggregate ;
  dcterms:identifier "Agg_1" ;
  rdfs:member apo:R7828 ;
  rdfs:member apo:R78520 ;
  rdfs:member apo:R78521 ;
  rdfs:member apo:R78522 ;
  rdfs:member apo:R78523 ;
.
auspix:R7852
  a apo:Cell ;
  apo:downNeighbour apo:R7855 ;
  apo:leftNeighbour apo:R7851 ;
  apo:rightNeighbour apo:R8630 ;
  apo:upNeighbour apo:R7828 ;
  geox:centroid "POINT (149.44444444444443 -35.23915910922053)"^^geo:wktLiteral ;
  geox:hasAreaM2 [
      data:value "12971551595"^^xsd:decimal ;
    ] ;
  dcterms:identifier "R7852" ;
  geo:hasGeometry "POLYGON ((148.88888888888889 -34.663795228918765, 150.0 -34.663795228918765, 150.0 -35.81859718358464, 148.88888888888889 -35.81859718358464))"^^geo:wktLiteral ;
  geo:sfContains apo:R78520 ;
  geo:sfContains apo:R78521 ;
  geo:sfContains apo:R78522 ;
  geo:sfContains apo:R78523 ;
  geo:sfContains apo:R78524 ;
  geo:sfContains apo:R78525 ;
  geo:sfContains apo:R78526 ;
  geo:sfContains apo:R78527 ;
  geo:sfContains apo:R78528 ;
  geo:sfWithin apo:R785 ;
.
<https://orcid.org/0000-0002-3884-3420>
  a sdo:Person ;
  sdo:affiliation <http://catalogue.linked.data.gov.au/org/csiro> ;
  sdo:email "simon.cox@csiro.au" ;
  sdo:identifier "https://orcid.org/0000-0002-3884-3420"^^xsd:anyURI ;
  sdo:mainEntityOfPage <https://people.csiro.au/C/S/simon-cox> ;
  sdo:name "Simon J D Cox" ;
  sdo:subjectOf <https://people.csiro.au/C/S/simon-cox> ;
.
